

We can again do it by substitution. I can solve for  $x$  in the second equation.

$$-x = 2 - 5y$$

$$x = -2 + 5y$$

Now substitute this expression in the 1<sup>st</sup> and 3<sup>rd</sup> equations.

$$1^{\text{st}} \text{ eqn: } 3(-2 + 5y) + 2y = 5 \Rightarrow -6 + 15y + 2y = 5 \Rightarrow 17y = 11$$

$$3^{\text{rd}} \text{ eqn: } 2(-2 + 5y) + 7y = 3 \Rightarrow -4 + 10y + 7y = 3 \Rightarrow 17y = 7$$

Contradiction  $\Rightarrow$  It is an inconsistent system.

Here the three lines intersect at 3 points forming a triangle.

Example

$$2x + 3y = 1$$

$$-4x - 6y = 3$$

$$3x + 2y = 5$$

Again by substitution, let's solve for  $x$  in the first equation.

$$2x = 1 - 3y \Rightarrow x = \frac{1}{2}(1 - 3y) \Rightarrow x = \frac{1}{2} - \frac{3}{2}y$$

Putting it in the 2<sup>nd</sup> equation

$$-4\left(\frac{1}{2} - \frac{3}{2}y\right) - 6y = -2 + 6y - 6y = 3$$

$$-2 + 0y = 3$$

$$-2 = 3 \quad \text{Contradiction}$$

We have an inconsistent system.

The first 2 lines are  $\parallel$  and the third one intersects both of them at 2 different points.